Make SwapProp reusable

theories/DSubSyn/lr_lemma.v
@@ -2,20 +2,13 @@ From iris.base_logic Require Import base_logic.
 From iris.proofmode Require Import tactics.
 From D.pure_program_logic Require Import weakestpre lifting.
 From iris.program_logic Require Import language.
-From D Require Import tactics proofmode_extra.
+From D Require Import tactics proofmode_extra swap_later_impl.
 From D.DSub Require Import rules synLemmas step_fv.
 From D.DSubSyn Require Import unary_lr_binding.
 
 Import uPred.
 
 Implicit Types (L T U: ty) (v: vl) (e: tm) (Γ : ctx).
-
-Class SwapProp (PROP: sbi) := {
-  impl_later : ∀ (P Q: PROP), (▷ P → ▷ Q) ⊢ ▷ (P → Q)
-}.
-
-Lemma impl_laterN n `{SwapProp PROP} (P Q: PROP) : (▷^n P → ▷^n Q) ⊢ ▷^n (P → Q).
-Proof. elim: n => [//|n IHn]. by rewrite impl_later IHn. Qed.
 
 Section Sec.
   Context `{!dsubSynG Σ} `{!SwapProp (iPropSI Σ)}.
@@ -470,32 +463,6 @@ Proof.
 Qed.
 
 Instance dsubSynG_empty: dsubSynG #[].
-
-Class CmraSwappable (M : cmraT) := {
-  (* TODO cmra_extend should really be cmra_extend_sep. *)
-  cmra_extend_included: ∀ n (mx : option M) z,
-    ✓{S n} mx → ✓{n} (z ⋅? mx) → ∃ z', ✓{S n} (z' ⋅? mx) ∧ z ≡{n}≡ z'
-}.
-
-(* Lemma impl_later {M : ucmraT} `{!CmraSwappable M} (P Q: uPred M) : (▷ P → ▷ Q) ⊢ ▷ (P → Q). *)
-Instance SwapCmra {M : ucmraT} `{!CmraSwappable M}: SwapProp (uPredSI M).
-Proof.
-  split.
-  unseal; split => /= -[//|n] x ? HPQ n' ? [x' ->] ?? HP.
-  specialize (HPQ (S n')); cbn in HPQ.
-  case: (cmra_extend_included n' (Some x) x'); last move => x'' [];
-    rewrite /= ?[_ ⋅ x]comm ?Some_validN //=.
-  - by eapply cmra_validN_le; eauto with lia.
-  - move => Hv Hnx'x''.
-    rewrite Hnx'x''. apply HPQ; eauto using cmra_included_l with lia.
-    rewrite /uPred_holds /=. by rewrite -Hnx'x''.
-Qed.
-
-Instance Swappable_iResUREmpty: CmraSwappable (iResUR #[]).
-Proof.
-  split. rewrite /iResUR /gid /= => n mx z Hvmx Hvzmx.
-  exists z; split_and! => // ??. by apply fin_0_inv.
-Qed.
 
 Corollary type_soundness e e' thp σ σ' T:
   ([] ⊢ₜ e : T) →
