theories/swap_later_impl.v
@@ -1,0 +1,38 @@
+From D Require Import tactics proofmode_extra.
+From iris.proofmode Require Import tactics.
+From iris.base_logic Require Import lib.iprop (* For gname *)
+     lib.saved_prop.
+
+Import uPred.
+
+Class SwapProp (PROP: sbi) := {
+  impl_later : ∀ (P Q: PROP), (▷ P → ▷ Q) ⊢ ▷ (P → Q)
+}.
+
+Lemma impl_laterN n `{SwapProp PROP} (P Q: PROP) : (▷^n P → ▷^n Q) ⊢ ▷^n (P → Q).
+Proof. elim: n => [//|n IHn]. by rewrite impl_later IHn. Qed.
+
+Class CmraSwappable (M : cmraT) := {
+  (* TODO cmra_extend should really be cmra_extend_sep. *)
+  cmra_extend_included: ∀ n (mx : option M) z,
+    ✓{S n} mx → ✓{n} (z ⋅? mx) → ∃ z', ✓{S n} (z' ⋅? mx) ∧ z ≡{n}≡ z'
+}.
+
+Instance SwapCmra {M : ucmraT} `{!CmraSwappable M}: SwapProp (uPredSI M).
+Proof.
+  split.
+  unseal; split => /= -[//|n] x ? HPQ n' ? [x' ->] ?? HP.
+  specialize (HPQ (S n')); cbn in HPQ.
+  case: (cmra_extend_included n' (Some x) x'); last move => x'' [];
+    rewrite /= ?[_ ⋅ x]comm ?Some_validN //=.
+  - by eapply cmra_validN_le; eauto with lia.
+  - move => Hv Hnx'x''.
+    rewrite Hnx'x''. apply HPQ; eauto using cmra_included_l with lia.
+    rewrite /uPred_holds /=. by rewrite -Hnx'x''.
+Qed.
+
+Instance Swappable_iResUREmpty: CmraSwappable (iResUR #[]).
+Proof.
+  split. rewrite /iResUR /gid /= => n mx z Hvmx Hvzmx.
+  exists z; split_and! => // ??. by apply fin_0_inv.
+Qed.
